

Governing eqn

1) mass Conservation $\Rightarrow \nabla \cdot \mathbf{u} = 0$

2) momentum Conservation $\Rightarrow \rho \left[\frac{D\mathbf{u}}{Dt} \right] = -\nabla p + \nabla \cdot \boldsymbol{\tau} - \rho_E (\nabla \phi)$

3) Poisson's eq $\Rightarrow -\epsilon \nabla^2 \phi = \rho_E = F_Z C$

4) PNP eq $\Rightarrow \frac{\partial C}{\partial t} + \nabla \cdot \left(C\mathbf{u} - D\nabla C - \frac{DC}{V_T} \nabla \phi \right) = 0$

5) Conformation tensor \Rightarrow

$$\frac{\partial \mathbf{A}}{\partial t} + \mathbf{u} \cdot \nabla \mathbf{A} - \mathbf{A} \cdot \nabla \mathbf{u} - \nabla \mathbf{u}^T \cdot \mathbf{A} = \frac{1 + \epsilon (\text{tr} \mathbf{A} - 3)}{\lambda} (\mathbf{I} - \mathbf{A})$$

Scaling parameters: $\bar{x} = \frac{x}{R} \quad | \quad \bar{t} = t \frac{U}{R}$

$\bar{\nabla} = \nabla R \quad | \quad \bar{j}_E = \frac{j_E}{F Z C_0} \quad | \quad \bar{c} = \frac{c}{C_0}$

$\bar{u} = \frac{u}{U} \quad | \quad \bar{\phi} = \frac{\phi}{V_T} \quad | \quad \bar{p} = \frac{p}{\rho U^2}$

where,

$\bar{v} = \frac{E R}{V_T} \quad | \quad E = \frac{2V}{L} \quad | \quad U = \frac{e V_T^2}{\eta R} \quad | \quad V_T = \frac{kT}{eZ}$

$\eta = \eta_s + \eta_p \quad | \quad \beta = \frac{\eta_s}{\eta_s + \eta_p}$

* Dimensionless parameters used :

$$Re = \frac{\rho R U}{\eta}$$

$$Wi = \frac{\lambda U}{R}$$

1) Continuity equation :

$$\nabla \cdot \mathbf{u} = 0$$

\Rightarrow

$$\frac{\bar{\nabla}}{R} \cdot \bar{\mathbf{u}} = 0 \quad \left. \vphantom{\frac{\bar{\nabla}}{R} \cdot \bar{\mathbf{u}} = 0} \right\} \boxed{\bar{\nabla} \cdot \bar{\mathbf{u}} = 0}$$

2) Momentum Conservation :

$$\rho \left[\frac{\partial u}{\partial t} + u \cdot \nabla u \right] = -\nabla p + \nabla \cdot \tau - \rho_E \nabla \phi$$

$$a) \rho \left[\frac{\partial u}{\partial t} + u \cdot \nabla u \right] \rightarrow \rho \left[\frac{\partial (\bar{u}U)}{\partial \left(\frac{r}{R} \right)} + \bar{u}U \cdot \frac{\nabla}{R} (\bar{u}U) \right]$$

$$\Rightarrow \rho \left[\frac{U^2}{R} \left(\frac{\partial \bar{u}}{\partial \bar{t}} \right) + \frac{U^2}{R} (\bar{u} \cdot \nabla \bar{u}) \right]$$

$$\Rightarrow \left[\frac{\rho U^2}{R} \left[\frac{\partial \bar{u}}{\partial \bar{t}} + \bar{u} \cdot \nabla \bar{u} \right] \right]$$

$$b) \nabla P \Rightarrow \frac{\bar{\nabla} \bar{P} (P U^2)}{R} \Rightarrow \left(\frac{P U^2}{R} \right) [\bar{\nabla} \bar{P}]$$

$$\nabla \cdot \mathbf{Z} \rightarrow \nabla \cdot (\mathbf{Z}_s + \mathbf{Z}_p)$$

PTT Model,

$$\mathbf{Z}_s = 2\eta_s \mathbf{S}$$

where;

$$\mathbf{S} = \frac{1}{2} [\nabla \mathbf{u} + \nabla \mathbf{u}^T]$$

and

for $\mathbf{Z}_p \Rightarrow$

$$\mathbf{Z}_p \left[1 + \frac{\varepsilon \lambda \text{tr}(\mathbf{Z}_p)}{\eta_p} \right] + \lambda \left[\frac{\partial \mathbf{Z}_p}{\partial t} + \mathbf{u} \cdot \nabla \mathbf{Z}_p - \mathbf{Z}_p \cdot \nabla \mathbf{u} - \nabla \mathbf{u}^T \cdot \mathbf{Z}_p \right] = 2\eta_p \mathbf{S}$$

We are using Conformation tensor,

$$\mathbf{Z}_p = \frac{\eta_p}{\lambda} (\mathbf{A} - \mathbf{I})$$

\Rightarrow

$$\nabla \cdot \mathbf{Z} = \nabla \cdot \mathbf{Z}_s + \nabla \cdot \mathbf{Z}_p$$

$$= \nabla \cdot (2\eta_s \mathbf{S}) + \nabla \cdot \left[\frac{\eta_p}{\lambda} (\mathbf{A} - \mathbf{I}) \right]$$

$$c) \nabla \cdot Z = \nabla (2n_s s) + \nabla \left[\frac{n_p}{\lambda} (A - I) \right]$$

$$s = \frac{1}{2} (\nabla u + \nabla u^T)$$

$$\nabla \cdot Z = 2n_s \nabla s + \frac{n_p}{\lambda} \nabla A$$

$$\bar{s} = \frac{U}{R} s$$

$$= 2n_s \frac{\bar{\nabla}}{R} \left(\frac{U}{R} \right) s + \frac{n_p}{\lambda} \frac{\bar{\nabla}}{R} A$$

$$= \frac{U}{R} \left[\frac{1}{2} (\bar{\nabla} u + \bar{\nabla} u^T) \right]$$

$$\Rightarrow \nabla \cdot Z = \left(\frac{U}{R^2} \right) 2n_s (\bar{\nabla} \bar{s}) + \left(\frac{1}{R} \right) \frac{n_p}{\lambda} (\bar{\nabla} A)$$

$$d) \int_E \nabla \phi \rightarrow \bar{P}_E(fzC_0) \cdot \frac{\bar{\nabla} \phi}{R} V_T$$

$$\Rightarrow \int_E \nabla \phi = \left(\frac{fzC_0 V_T}{R} \right) \bar{P}_E \bar{\nabla} \phi$$

put everything in the eqn \Rightarrow

$$\Rightarrow \frac{SU^2}{R} \left[\frac{D\bar{U}}{D\bar{E}} \right] = - \frac{SU^2}{R} [\bar{\nabla}\bar{P}] + \frac{U}{R^2} 2n_s(\bar{\nabla}\bar{S}) + \frac{1}{R} \frac{n_p}{\lambda} (\bar{\nabla}A) - \frac{FZC_0V_T}{R} (\bar{f}_E \bar{\nabla}\bar{\phi})$$

$$\frac{D\bar{U}}{D\bar{E}} = -\bar{\nabla}\bar{P} + \frac{(2n_s U^2 / R^2)}{(SU^2/R)} \bar{\nabla}\bar{S} + \frac{(n_p / \lambda R)}{(SU^2/R)} (\bar{\nabla}A) - \left[\frac{FZC_0KT \times 1}{ReZ (SU^2/R)} \right] \bar{f}_E \bar{\nabla}\bar{\phi}$$

$$\frac{D\bar{U}}{D\bar{E}} = -\bar{\nabla}\bar{P} + \left[\frac{2n_s}{SUR} \times \frac{n}{\lambda} \right] \bar{\nabla}\bar{S} + \left[\frac{n_p}{SU^2 \lambda} \times \frac{n}{\lambda} \times \frac{R}{R} \right] \bar{\nabla}A - \left[\frac{FZC_0KT}{eZ \rho \left(\frac{eV_T^2}{\lambda R} \right) U} \right] \bar{f}_E \bar{\nabla}\bar{\phi}$$

$$\frac{D\bar{U}}{D\bar{E}} = -\bar{\nabla}\bar{P} + \left[\frac{2(n_s)(n)}{(n)(SUR)} \right] \bar{\nabla}\bar{S} + \left[\left(\frac{n_p}{n} \right) \left(\frac{n}{SUR} \right) \left(\frac{R}{\lambda U} \right) \right] \bar{\nabla}A - \left[\frac{FZC_0}{\rho (KT/eZ) \times e^{\frac{h^* R}{U}} \times \frac{R}{R}} \right] \bar{f}_E \bar{\nabla}\bar{\phi} \times \frac{2}{2}$$

$$\Rightarrow \frac{D\bar{u}}{D\bar{t}} = -\bar{\nabla}\bar{p} + \frac{2\beta}{Re}(\bar{\nabla}\bar{s}) + \frac{(1-\beta)}{(Re)(Wi)} \times \bar{\nabla}A$$

$$- \left(\frac{2FeZ^2 C_0 R^2}{\epsilon_{KT}} \right) \times \left(\frac{\eta}{\beta_{UR}} \right) \times \left[\frac{\bar{p}_E \bar{\nabla}\bar{\phi}}{2} \right]$$

K^2 (given)

$$\Rightarrow \frac{D\bar{u}}{D\bar{t}} = -\bar{\nabla}\bar{p} + \frac{2\beta}{Re}(\bar{\nabla}\bar{s}) + \frac{(1-\beta)}{(Re)(Wi)} \times \bar{\nabla}A$$

$$- \frac{K^2}{2Re} (\bar{p}_E \bar{\nabla}\bar{\phi})$$

3) Poisson's eqn:

$$-\epsilon \nabla^2 \phi = \rho_c = FZC$$

$$-\nabla^2 \phi = \frac{FZC}{\epsilon}$$

$$\Rightarrow -\frac{\nabla^2 \phi}{R^2} \left(\frac{V_T}{V_T} \right) = \frac{FZ\bar{C}_0}{\epsilon}$$

$$\Rightarrow \nabla^2 \phi = \frac{FZ\bar{C}_0}{\epsilon} \left(\frac{R^2}{V_T} \right)$$

$$= \frac{FZ\bar{C}_0}{\epsilon} \times \frac{R^2}{(kT/e)} = \frac{FZ\bar{C}_0 R^2}{\epsilon kT}$$

$$\Rightarrow \nabla^2 \phi = \frac{FZ\bar{C}_0 R^2}{\epsilon kT} = -\left(\frac{FZ\bar{C}_0 R^2}{\epsilon kT} \right) \frac{e}{2}$$

$$\Rightarrow \nabla^2 \phi = -\left(\frac{k^2}{2} \right) \bar{C}$$

\downarrow
 $= k$
 (given in paper)

4) PNP eqn

$$\frac{\partial c}{\partial t} + \nabla \cdot (c\mathbf{u} - D\nabla c - \frac{D}{V_T} c \nabla \phi) = 0$$

$$\Rightarrow \frac{\partial(\bar{c}_0)}{\partial(\bar{t} R/V)} + \frac{\bar{\nabla}}{R} \cdot (\bar{c}_0 \bar{u} V - D \frac{\bar{\nabla}}{R} \bar{c}_0 - \frac{D}{V_T} \bar{c}_0 \frac{\bar{\nabla}}{R} \bar{\phi} V_T) = 0$$

$$\Rightarrow \cancel{R} V \left(\frac{\partial \bar{c}}{\partial \bar{t}} \right) + \bar{\nabla} \cdot (\cancel{c}_0) \left(\bar{c} \bar{u} V - D \frac{\bar{\nabla}}{R} \bar{c} - D \bar{c} \frac{\bar{\nabla}}{R} \bar{\phi} \right) = 0$$

$$\Rightarrow \frac{\partial \bar{c}}{\partial \bar{t}} + \bar{\nabla} \cdot \left[\bar{c} \bar{u} - \left(\frac{D}{RV} \right) \bar{\nabla} \bar{c} - \left(\frac{D}{RV} \right) \bar{c} \bar{\nabla} \bar{\phi} \right] = 0$$

1 TUE
DAY 172-193

$$\Rightarrow \frac{D}{RV} = \frac{1}{Pe} \quad (\text{Peclet no.})$$

$$\Rightarrow \boxed{\frac{\partial \bar{c}}{\partial \bar{t}} + \bar{\nabla} \cdot \left[\bar{c} \bar{u} - \frac{1}{Pe} \bar{\nabla} \bar{c} - \frac{1}{Pe} \bar{c} \bar{\nabla} \bar{\phi} \right] = 0}$$

5) Conformation tensor ($A \rightarrow$ dimensionless)

$$\frac{\partial A}{\partial t} + u \cdot \nabla A - A \cdot \nabla u - \nabla u^T \cdot A = \frac{1 + \epsilon(\text{tr} A - 3)}{\lambda} (I - A)$$

$$\Rightarrow \frac{\partial A}{\partial(\bar{t} R U)} + \bar{u} \cdot \frac{\nabla A}{R} - A \cdot \frac{\nabla \bar{u}}{R} - \frac{\nabla \bar{u}^T}{R} \cdot A = \frac{1 + \epsilon(\text{tr} A - 3)}{\lambda} (I - A)$$

$$\Rightarrow \frac{U}{R} \left[\frac{\partial A}{\partial \bar{t}} + \bar{u} \cdot \nabla A - A \cdot \nabla \bar{u} - \nabla \bar{u}^T \cdot A \right] = \frac{1 + \epsilon(\text{tr} A - 3)}{\lambda} (I - A)$$

$$\Rightarrow \frac{\partial A}{\partial \bar{t}} + \bar{u} \cdot \nabla A - A \cdot \nabla \bar{u} - \nabla \bar{u}^T \cdot A = \frac{1 + \epsilon(\text{tr} A - 3)}{\lambda U} (I - A) \times \left(\frac{R}{\lambda U} \right)$$

\downarrow
 w_i

$$\Rightarrow \boxed{\frac{\partial A}{\partial \bar{t}} + \bar{u} \cdot \nabla A - A \cdot \nabla \bar{u} - \nabla \bar{u}^T \cdot A = \frac{1 + \epsilon(\text{tr} A - 3)}{w_i} (I - A)}$$